Multisem/Text/Macros.lean
@@ -1,0 +1,50 @@
+import Lean
+import Lean.Syntax
+open Lean Meta Std
+
+inductive tree (A:Type) where
+  | one : A -> tree A
+  | comp : tree A -> tree A -> tree A
+instance {A:Type} : Coe A (tree A) where
+  coe a := tree.one a
+notation:64 x "#" y => tree.comp x y
+
+def buildAppend (stx: Lean.Syntax) (l:List Lean.Syntax) : Lean.MacroM (Lean.TSyntax `term) :=
+  match l with
+  | [] => throw (Lean.Macro.Exception.error stx "Must have at least one word")
+  | x::[] => match x with
+             | Lean.Syntax.ident _ _ (Lean.Name.str _ txt) _ =>
+               pure (Lean.Syntax.mkCApp `tree.one #[Lean.Syntax.mkStrLit txt])
+               --pure (Lean.Syntax.mkCApp `List.cons #[Lean.Syntax.mkStrLit txt, Lean.Syntax.mkCApp `List.nil #[]])
+               --pure (Lean.Syntax.node Lean.SourceInfo.none `Lean.Parser.)
+               --pure (mkApp (mkApp (mkConst `List.cons) (mkStrLit txt)) (mkConst `List.empty))
+               --(Lean.Syntax.node Lean.SourceInfo.none 
+               --       `List.cons #[(Lean.Syntax.mkStrLit txt) `List.empty])
+             | _ => --pure (Lean.Syntax.mkStrLit (toString x))
+               throw  (Lean.Macro.Exception.error stx "Only individual words are valid")
+  | x::xs => 
+    do
+      let rhs <- buildAppend stx xs;
+      match x with
+      | Lean.Syntax.ident _ _ (Lean.Name.str _ txt) _ =>
+        pure (Lean.Syntax.mkCApp `tree.comp #[Lean.Syntax.mkStrLit txt, rhs])
+      | _ => throw (Lean.Macro.Exception.error stx "Only individual words are valid")
+
+syntax (name := splitParser) "[|" ident+ "|]": term
+@[macro splitParser] def implSplitParser : Lean.Macro :=
+  fun stx =>
+    let val := stx;
+    let argc := Lean.Syntax.getNumArgs val;
+    let text := Lean.Syntax.getArg val 1;
+    --let stext := toString text;
+    --let words := String.splitOn stext " ";
+    do
+      --let info <- Lean.MonadRef.mkInfoFromRefPos;
+      match text with
+      | Lean.Syntax.node _ _ mid => buildAppend val mid.data
+      | _ => pure (Lean.Syntax.mkNumLit (toString argc))
+      --pure (Lean.Syntax.mkStrLit stext)
+def blahh := [| four equals four |]
+#print blahh
+--#eval blahh
+theorem blahhh : blahh = "four"#("equals"#"four") := by rfl
